\documentclass[../diffeq.tex]{subfiles}
\graphicspath{{\subfix{../figures/}}}
\begin{document}
\chapter{Linear Second-Order Equations}
\section{Introduction: The Mass-Spring Oscillator}
A damped mass-spring oscillator consists of a mass $m$ attached to a spring fixed at one end. Devise a differential equation that governs the motion of this oscillator, taking into account 
the forces acting on it due to the spring elasticity, damping friction, and possible external influences.

Newton's second law - force equals mass times acceleration ($F=ma$) - is the most commonly encountered differential equation. It is an ordinary differential equation of the second order 
since acceleration is the second derivative of position ($y$) with respect to time ($a=\dd^2 y/\dd t^2$).

If the spring is unstretched and the inertial mass $m$ is still, the system is at equilibrium. We stretch the coordinate $y$ of the mass by its displacement from the equilibrium position.

When the mass $m$ is displaced from equilibrium, the spring is stretched or compressed and it exerts a force that resists the displacement. For most springs this force is directly proportional to the displacement $y$ 
and is given by Hooke's law.
\[ F_{\text{spring}}= -ky \]
where the positive constant $k$ is known as the stiffness (spring constant) and the negative sign reflects the opposing nature of the force. Hooke's law is only valid for sufficiently small displacements.

Usually all mechanical systems also experience friction. For vibrational motion this force is usually modeled accurately by a term proportional to velocity:
\[ F_{\text{friction}}=-b\frac{\dd y}{\dd t}=-by' \]
where $b\geq 0$ is the damping coefficient and the negative sign reflects the opposing nature of the force.

The other forces on the oscillator are usually regarded as external to the system. Although they may be gravitational, electrical, or magnetic, commonly the most important external forces are transmitted 
to the mass by shaking the supports holding the system. For now we refer to the combined external forces by a single known function $F_{\text{ext}}(t)$. Newton's law provides the differential equation for the mass-spring oscillator:
\[ my''=-ky-by'+F_{\text{ext}}(t)\] or \[ my''+by'+ky=F_{\text{ext}}(t) \]

\begin{example}
    Verify that if $b=0$ and $F_{\text{ext}}=0$, that the above equation has a solution of the form $y(t)=\cos(\omega t)$ and the angular frequency $\omega$ increases with $k$ and decreases with $m$.

    The differential equation is $my''+by'+ky=F_{\text{ext}}$ and that $my''+ky=0$.

    Since we are given what $y(t)$ is, taking the derivative of the differential equation gives that $-m\omega^2\cos(\omega t)+k\cos(\omega t)=0$, and solving for $\omega$, we get that $\omega=\sqrt{\frac{k}{m}}$.

    If $k$ increases, $\omega$ increases, and if $m$ increases, $\omega$ decreases.
\end{example}

\begin{example}
    Verify that the exponentially damped sinusoid given by $y(t)=e^{-3t}\cos 4t$ is a solution to the above differential equation if $F_{\text{ext}}=0, m=1, k=25$, and $b=6$.

    From the differential equation $my''+by'+ky=F_{\text{ext}}$, we can plug in stuff and we get that $y''+by'+25y=0$.

    Since we are given $y(t)$ we can find the derivatives and substitute. What we are given is quite long, but essentially it cancels out to $0=0$, which means it is a solution to the system.
\end{example}

\ex Verify that the simple exponential function $y(t)=e^{-5t}$ is a solution to the above differential equation if $F_{\text{ext}}=0$, $m=1$, $k=25$, and $b=10$.

Sometimes the external force will make the system look somewhat erratic. There are many real world examples where the external force must defintely be taken into account.

\section{Homogeneous Linear Equations: The General Solution}
A second-order constant-coefficient differential equation has the form 
\[ ay''+by'+cy=f(t) \qquad (a\neq 0) \]
A homogeneous second-order constant-coefficient differential equation is the special case with $f(t)=0$.
\[ ay''+by'+cy=0 \qquad (a\neq 0) \]
A solution of this equation has the form $y=e^{rt}$. The resulting equation $ar^2+br+c=0$ is called the auxiliary equation (or characteristic equation) associated with the homogeneous equation.

\begin{example}
    Find a pair of solutions to 
    \[ y''+5y'-6y=0\]

    Plugging in $y=e^{rt}$, we get that $e^{rt}(r^2+5r-6)$ after substituting. Solving the quadratic $r^2+5r-6 =0$, we get that $r=-6$ and $r=1$, which is $y=e^{-6t}$ and $y=e^t$.
\end{example}

Note that the zero function, $y(t)=0$ is always a solution to an equation above (figure this out later). In addition when we have a pair of solutions $y_1(t)$ and $y_2(t)$, we can construct an infinite number of other solutions by forming linear combinations:
\[ y(t)=c_1y_1(t)+c_2y_2(t) \]
for any choice of the constants $c_1$ and $c_2$. This is a two-paramter solution form since there are two unknown constants. To find a specific solution, two initial conditions are needed.

\begin{example}
    Solve the initial value problem 
    \[ y''+2y'-y=0\qquad y(0)=0, \qquad y'(0)=-1 \]

    Doing the default substitution, our auxiliary equation is $r^2+2r-1=0$. 

    The solutions from this are $r=-1+\sqrt{2}$ and $r=-1-\sqrt{2}$. Remember $y=e^{rt}$. Using the initial conditions, we get that $c_1=-\frac{\sqrt{2}}{4}$ and $c_2=\frac{\sqrt{2}}{4}$.
\end{example}

\begin{theorem}
    For any real numbers $a(\neq 0),b,c,t_0,Y_0$, and $Y_1$, there exists a unique soultion to the initial value problem. 
    \[ ay''+by'+cy=0 \qquad y(t_0)=Y_0 \qquad y'(t_0)=y_1 \]
    The solution is valid for all $t$ in $(-\infty,\infty)$
\end{theorem}

\begin{definition}
    A pair of functions $y_1(t)$ and $y_2(t)$ is said to be linearly independent on the interval $t$ if and only if neither of them is a constant multiple of the other on all of $t$. We say that 
    $y_1$ and $y_2$ are linearly dependent on $t$ if one of them is a constant multiple of the other on all of $t$.
\end{definition}

\begin{theorem}
    If $y_1(t)$ and $y_2(t)$ are any two solutions to the differential equation that are linearly independent on $(-\infty,\infty)$, then unique constants $c_1$ and $c_2$ can always be found so that $c_1y_1(t)+c_2y_2(t)$ satisfies the initial value problem on $(-\infty,\infty)$.
\end{theorem}

\begin{definition}[Wronksian]
    Suppose each of the functions $f_1(x),f_2(x),\dots f_n(x)$ possess at least $n-1$ derivatives. 
    
    The determinant \[
        W(f_1, f_2, \dots, f_n) =
        \begin{vmatrix}
        f_1 & f_2 & \dots & f_n \\
        f_1' & f_2' & \dots & f_n' \\
        \vdots & \vdots & \ddots & \vdots \\
        f_1^{(n-1)} & f_2^{(n-1)} & \dots & f_n^{(n-1)}
        \end{vmatrix}
        \]
        is called the Wronksian of the functions.
\end{definition}

\begin{theorem}
    Let $y_1,y_2,\dots,y_n$ be $n$ solutions of the homogeneous linear $n$th-order differential equation on an interval $I$. Then the set of solutions is linearly independent on $I$ 
    if and only if $W(y_1,y_2,\dots,y_n)\neq 0$ for every $x$ in the interval.
\end{theorem}

Distinct real roots: If the auxiliary equation has distinct real roots $r_1$ and $r_2$, then both $y_1(t)=e^{rt}$ and $y_2(t)=e^{rt}$ are solutions to the above differential equation and $y(t)=e_1e^{rt}+e_2e^{rt}$ is a general solution.

Repeated root: if the auxiliary equation has a repeated root $r$, then both $y_1(t)=e^{rt}$ and $y_2(t)=te^{rt}$ are solutions to the differential equation and $y(t)=e_1e^{rt}+e_2te^{rt}$ is a general solution.

A homogeneous linear $n$th-order equation has a general solution of the form 
\[ y(t)=c_1y_1(t)+c_2y_2(t)+\dots+c_ny_n(t) \]
where the individual solutions $y_i(t)$ are linearly independent, i.e. no $y_i(t)$ is expressible as a linear combination of the others.

\section{Auxiliary Equations with Complex Roots}
The simple harmonic equation $y''+y=0$ so called because of its relation to the fundamental vibration of a musical tone, has as solutions $y_1(t)=\cos t$ and $y_2(t)=\sin t$.

When $b^2-4ac<0$, the roots of the auxiliary equation $ar^2+br+c=0$ associated with the homogeneous equation $ay''+by'+cy=0$ are the complex conjugate numbers $r_1=\alpha + i\beta$ and $r_2=\alpha-i\beta$ where $\alpha=-\frac{b}{2a}$ and $\beta = \frac{\sqrt{4ac-b^2}}{2a}$

Combing the solutions $e^{r_1t}$ and $e^{r_2t}$ with Euler's formula $e^{i\theta}=\cos\theta + i\sin\theta$, yields complex function solutions 
\[ e^{(\alpha+i\beta)t}=e^{at}(\cos\beta t+i\sin\beta t) \text{ and } e^{(\alpha-i\beta)t}=e^{at}(\cos\beta t-i\sin\beta t) \]

\begin{example}
    Solve the initial value problem $y''+2y'+2y=0$ given $y(0)=0$ and $y'(0)=2$.

    Using the auxiliary form of the equation we have $r^2+2r+2=0$. From the quadratic formula, $r=-1\pm i$, the two roots are $r_1=-1+i$ and $r_2=-1-i$.

    The solution is therefore $y_1=e^{(-1+i)t}$ and $y_2=e^{(-1-i)t}$

    From the form given from euler's formula earlier, $y_1=e^{-t}(\cos t+i\sin t)$ and $y_2=e^{-t}(\cos t-i\sin t)$, so our general solution is $y=c_1e^{-t}(\cos t+i\sin t)+c_2e^{-t}(\cos t-i\sin t)$.

    Plugging the initial conditions, we get that $0=c_1+c_2$.

    The derivative of the general solution is $y'=c_1e^{-t}(-\sin t+i\cos t)+(\cos t+i\sin t)\cdot c_1(-1)e^{-t}+c_2e^{-t}(-\sin t-i\cos t)+(\cos t-i\sin t)\cdot c_2(-1)e^{-t}$. Plugging in the initial conditions gives $2=c_1i-c_1-c_2i-c_2$.

    Factoring we get $2=c_1(i-1)+c_2(-i-1)$. Using some substitution $c_2=i$ and $c_1=-i$. Plug this in the general solution to solve.
\end{example}

If the auxiliary equation has complex conjugate roots $a\pm i\beta$, then two linearly independent solutions to the equation are 
\[ e^{\alpha t}\cos \beta t \text{ and } e^{\alpha t}\sin \beta t\]
and a general solution is 
\[ y(t)=c_1e^{\alpha t}\cos \beta t + c_2e^{\alpha t}\sin \beta t \]
where $c_1$ and $c_2$ are arbitrary constants.

\begin{example}
    Find a general solution to $y''+2y'+4y=0$.

    Using the auxiliary equation the roots are $-1\pm \sqrt{3}i$. Using what was given above, the general solution is $y=c_1e^{-t}\cos(\sqrt{3}t)+c_2e^{-t}\sin(\sqrt{3}t)$.
\end{example}

\begin{example}
    Newton's second law implies the position $y(t)$ of the mass $m$ is governed by the second-order differential equation $my''(t)+by'(t)+ky(t)=0$ where the terms are physically identified as $my$ being interial, $by$ is damping and $ky$ is stiffness.
    Determine the equation of motion for a spring system when $m=36$ kg, $b$ = 12 kg/sec (which is equivalent to 12 N - sec/m), $k=37$ kg/sec$^2$, $y(0)=0.7$ m and $y'(0) = 0.1$ m/sec. Also find $y(10)$, the displacement after 10 sec.

    The differential equation is $36y''+12y'+37$, so the roots are $-\frac{1}{6}\pm i$.

    Doing the methods explained above, the solution is $y=.7e^{-t/6}\cos t + \frac{13}{60}e^{-t/6}\sin t$, and $y(10)\approx -.13$ m.
\end{example}
\ex Interpret the equation $y''+5y'-6y=0$ in terms of the mass-spring system.

\section{Nonhomogeneous Equations: the Method of Undetermined Coefficients}
The method of Undetermined Coefficients is the technique used to guess a solution's form based on the form of the nonhomogeneous function $f(t)$ in a linear equation with 
constant coefficients such as $ay''+by'+cy=f(t)$.

For example the particular solution to $ay''+by'+cy=Ct^m$ is of the form $y_p(t)=A_mt^m+\dots+A_1t+A_0$.

\begin{example}
    Find a particular solution to $y''+3y'+2y=10e^{3t}$.

    Our guess based on the form of $f(t)=10e^{3t}$ is that $y=Ae^{3t}$ is the guess form of the particular solution, so we know that $y'=3A3^{3t}$ and $y''=9Ae^{3t}$.

    Substituting this in gives us $9Ae^{3t}+3(3Ae^{3t})+2(Ae^{3t})=10e^{3t}$. Simplifying this gives us $20Ae^{3t}=10e^{3t}$ so $A=1/2$.

    So our particular solution is $\frac{1}{2}e^{3t}$.
\end{example}

\begin{example}
    Find a particular solution to $y''+3y'+2y=\sin t$.

    Let $y=A\sin t + B\cos t$ as the form of the particualr solution.

    Substituting and solving should result in $A=1/10$ and $B=-3/10$. 
\end{example}

This example suggests an equation of the form $ay''+by'+cy=C\sin\beta t$ (or $C\cos\beta t$) will have a particular solution of the form $y_p(t)=A\cos\beta t+B\sin\beta t$.

\begin{example}
    Find a particular solution to $y''+4y=5t^2e^t$.

    Let $y= At^2e^t+Bte^t+Ce^t = e^t(At^2+Bt+C)$. The result should be $A=1,B=-4/5, C=-2/25$.
\end{example}

To find a particular soultion to the differential equation 
\[ ay''+by'+cy=Ct^me^{rt} \]
where $m$ is a nonnegative integer, use the form 
\[ y_p(t)=t^s(A_mt^m+\dots +A_1t+A_0)e^{rt} \]
with 
\begin{enumerate}
    \item $s=0$ if $r$ is not a root of the associated auxiliary equation;
    \item $s=1$ if $r$ is a simple root of the associated auxiliary equation;
    \item $s=2$ if $r$ is a double root of the associated auxiliary equation.
\end{enumerate}

To find a solution to the differential equation $ay''+by'+cy = Ct^me^{\alpha t}\cos \beta t$ or equal to $Ct^me^{\alpha t}\sin\beta t$ for $\beta \neq 0$, use the form $y_p(t)=t^s(A_mt^m+\dots A_1t+A_0)e^{\alpha t}\cos\beta t+t^s(B_mt^m+\dots +B_1t+B_0)e^{\alpha t}\sin\beta t$, with 
\begin{enumerate}
    \item $s=0$ if $\alpha + i\beta$ is not a root of the associated auxiliary equation; and 
    \item $s=1$ if $\alpha + i\beta$ is a root of the associated auxiliary equation
\end{enumerate}

\section{The Superposition Principle and Undetermined Coefficients Revisited}
\section{Variation of Parameters}
\section{Variable-Coefficient Equations}

\end{document}